Queue_set

inductive_proof/Queue_set/App.fst
@@ -40,44 +40,32 @@ let get_ele (o:op_t{Enqueue? (fst (snd o))}) : nat =
   match o with
   |(_, (Enqueue x,_)) -> x
 
-let check_find_min (s:concrete_st)
-  : Lemma (requires s = S.add (2,1) (S.singleton (3,1)))
-          (ensures S.find_min s = Some (2,1)) 
-  = let m = S.find_min s in
-    assert (S.mem (2,1) s /\ (forall e1. S.mem e1 s ==> fst (2,1) <= fst e1));
-    (*assert (Some? m);
-    assert (fst (extract_s m) = 1);
-    assert (forall e. mem e s ==> 1 <= fst e);*) ()
-
-// apply an operation to a state
-let do (s:concrete_st) (op:op_t) : concrete_st =
-  match op with
-  |(id, (Enqueue x, _)) -> S.add (id, x) s
-  |(_, (Dequeue, _)) -> if s = S.empty then s else S.remove_min s
-
-let eq_min_same (a b:concrete_st) 
-  : Lemma (requires eq a b /\ S.unique_st a /\ S.unique_st b)
-          (ensures S.find_min a = S.find_min b) = ()
-
-let lem_do (a b:concrete_st) (op:op_t)
-   : Lemma (requires eq a b)
-           (ensures eq (do a op) (do b op)) = 
-  assume (S.unique_st a /\ S.unique_st b);
-  if Enqueue? (fst (snd op)) then () else ()
-  
 let return (s:concrete_st) (o:op_t) : ret_t =
   match o with
   |(_, (Enqueue _, _)) -> None
   |(_, (Dequeue, r)) -> if s = S.empty then None 
                           else (S.always_min_exists s; 
                                 assert (Some? (S.find_min s));
-                                Some (S.extract_s (S.find_min s)))
+                                Some (S.extract (S.find_min s)))
+                                
+// apply an operation to a state
+let do (s:concrete_st) (op:op_t{do_pre s op}) : concrete_st =
+  match op with
+  |(id, (Enqueue x, _)) -> S.add (id, x) s
+  |(_, (Dequeue, _)) -> if s = S.empty then s else S.remove_min s
+
+let lem_do (a b:concrete_st) (op:op_t)
+   : Lemma (requires eq a b /\ do_pre a op /\ do_pre b op)
+           (ensures eq (do a op) (do b op)) = 
+  if Enqueue? (fst (snd op)) then () else ()
 
 let last_deq (s:concrete_st) (op:op_t)
-  : Lemma (requires true)
-          (ensures (Dequeue? (fst (snd op)) /\ Some? (ret_of op) /\ return s op == ret_of op) ==>
+  : Lemma (requires true)         
+          (ensures ((Dequeue? (fst (snd op)) /\ Some? (ret_of op) /\ return s op == ret_of op) ==>
                    s <> S.empty /\ S.find_min s == ret_of op /\
-                   S.mem (S.extract_s (S.find_min s)) s) =
+                   S.mem (S.extract (S.find_min s)) s) /\
+                   (Dequeue? (fst (snd op)) /\ None? (ret_of op) /\ return s op == ret_of op ==> s = S.empty) /\
+                   ((s <> S.empty /\ Dequeue? (fst (snd op)) /\ ret_of op == return s op) ==> Some? (ret_of op))) =
   S.always_min_exists s
 
 let ret_ele (o:op_t{Dequeue? (fst (snd o)) /\ Some? (ret_of o)}) : (pos * nat) =
@@ -93,67 +81,56 @@ let resolve_conflict (x:op_t) (y:op_t{fst x <> fst y}) : resolve_conflict_res =
   |(_,(Enqueue _,_)), (_,(Dequeue,Some _)) -> First_then_second
   |(_,(Dequeue,Some _)), (_,(Enqueue _,_)) -> Second_then_first 
   |(_,(Dequeue,Some _)), (_,(Dequeue,Some _)) -> if ret_ele x = ret_ele y then First 
-                                                 else if fst (ret_ele x) > fst (ret_ele y) then First_then_second
+                                                 else if fst (ret_ele x) >= fst (ret_ele y) then First_then_second
                                                       else Second_then_first
- 
+
 let concrete_merge (lca s1 s2:concrete_st) 
   : Pure concrete_st
-         (requires (exists l1 l2. apply_log lca l1 == s1 /\ apply_log lca l2 == s2))
+         (requires true) // (exists l1 l2. apply_log lca l1 == s1 /\ apply_log lca l2 == s2))
          (ensures (fun _ -> True)) =
-  let i' = S.intersect s1 s2 in
-  let i = S.intersect lca i' in
+  let i = S.intersect lca (S.intersect s1 s2) in
   let da = S.remove_if s1 (fun e -> S.mem e lca) in
   let db = S.remove_if s2 (fun e -> S.mem e lca) in
   let m = S.union i (S.union da db) in
   m
 
-let merge_min (lca s1 s2:concrete_st) (m:(pos & nat))
-  : Lemma (requires (exists l1 l2. apply_log lca l1 == s1 /\ apply_log lca l2 == s2) /\
-                    Some? (S.find_min (concrete_merge lca s1 s2)) /\
-                    m = S.extract_s (S.find_min (concrete_merge lca s1 s2)))
-          (ensures S.mem m s1 \/ S.mem m s2) = 
-  S.always_min_exists lca; S.always_min_exists s1; S.always_min_exists s2
+let merge_prop (lca s1 s2:concrete_st) 
+  : Lemma (forall e. S.mem e (concrete_merge lca s1 s2) <==>               
+                ((S.mem e lca /\ S.mem e s1 /\ S.mem e s2) \/
+                 (S.mem e s1 /\ not (S.mem e lca)) \/
+                 (S.mem e s2 /\ not (S.mem e lca))) /\
+          (forall e. (S.mem e (concrete_merge lca s1 s2) /\ S.mem e lca /\ S.mem e s2) ==> S.mem e s1)) = ()
 
-let do_is_unique (s:concrete_st) (op:op_t) 
-  : Lemma (requires S.unique_st s /\ (not (S.mem_id_s (fst op) s)))
-          (ensures S.unique_st (do s op)) = 
-  match op with
-  |(id, (Enqueue x, _)) -> ()
-  |(_, (Dequeue, _)) -> ()
-
-let append_id (l:concrete_st) (ele:(pos * nat))
-  : Lemma (ensures (forall id. S.mem_id_s id (S.add ele l) <==> S.mem_id_s id l \/ id = fst ele) /\
-                   (S.unique_st l /\ not (S.mem_id_s (fst ele) l)) ==> 
-                    S.unique_st (S.add ele l))
-  = ()
+let merge_prop1 (lca s1 s2:concrete_st) (mini:(pos & nat)) 
+  : Lemma (requires S.find_min (concrete_merge lca s1 s2) = Some mini /\
+                    S.mem mini lca /\ S.mem mini s1 /\ S.mem mini s2 /\
+                    S.unique_st lca /\ S.unique_st s1 /\ S.unique_st s2)         
+          (ensures S.find_min (S.intersect lca (S.intersect s1 s2)) = Some mini) = ()
 
 let rec lem_foldl (s:concrete_st) (l:log)
-  : Lemma (requires true)
+  : Lemma (requires apply_log_ret s l)
           (ensures (forall id. S.mem_id_s id (apply_log s l) ==> S.mem_id_s id s \/ mem_id id l) /\
                    (forall e. S.mem e (apply_log s l) ==> S.mem e s \/ 
-                         (exists op. mem op l /\ (*Enqueue? (fst (snd op)) /\*) e == (fst op, get_ele op))))
+                         (exists op. mem op l /\ e == (fst op, get_ele op))))
           (decreases length l) =
   match length l with
   |0 -> ()
-  |_ -> (if Enqueue? (fst (snd (head l))) then append_id s (fst (head l), get_ele (head l)) else ());
-       mem_cons (head l) (tail l);
+  |_ -> mem_cons (head l) (tail l);
        lem_foldl (do s (head l)) (tail l)
        
 let rec lem_foldl1 (s:concrete_st) (l:log)
-  : Lemma (requires S.unique_st s /\ distinct_ops l /\
+  : Lemma (requires apply_log_ret s l /\ S.unique_st s /\ distinct_ops l /\
                     (forall id. S.mem_id_s id s ==> not (mem_id id l)))
           (ensures S.unique_st (apply_log s l))
           (decreases length l) =
   match length l with
   |0 -> ()
-  |_ -> do_is_unique s (head l);
-       (if Enqueue? (fst (snd (head l))) then append_id s (fst (head l), get_ele (head l)) else ());
-       mem_cons (head l) (tail l);
+  |_ -> mem_cons (head l) (tail l);
        distinct_invert_append (create 1 (head l)) (tail l);
-       lem_foldl1 (do s (head l)) (tail l)
+       lem_foldl1 (do s (head l)) (tail l); ()
 
 let valid_is_unique (s:st0) 
-  : Lemma (requires distinct_ops (ops_of s) /\ v_of s == apply_log init_st (ops_of s))
+  : Lemma (requires apply_log_ret init_st (ops_of s) /\ distinct_ops (ops_of s) /\ v_of s == apply_log init_st (ops_of s))
           (ensures S.unique_st (v_of s)) =
   lem_foldl1 init_st (ops_of s)
 
@@ -165,20 +142,25 @@ let merge_is_comm (lca s1 s2:st)
                        (concrete_merge (v_of lca) (v_of s2) (v_of s1)))) = ()
   
 let linearizable_s1_0''_base_base (lca s1 s2':st) (last2:op_t)
-  : Lemma (requires consistent_branches lca s1 (do_st s2' last2) /\
+  : Lemma (requires apply_log_ret init_st (snoc (ops_of s2') last2) /\
+                    consistent_branches lca s1 (do_st s2' last2) /\
                     ops_of s1 = ops_of lca /\ ops_of s2' = ops_of lca /\
                     length (ops_of lca) = 0)
         
           (ensures eq (do (v_of s2') last2) (concrete_merge (v_of lca) (v_of s1) (do (v_of s2') last2))) = ()
 
 let linearizable_s1_0''_base_ind (lca s1 s2':st) (last2:op_t)
-  : Lemma (requires consistent_branches lca s1 (do_st s2' last2) /\
+  : Lemma (requires apply_log_ret init_st (snoc (ops_of s2') last2) /\
+                    do_pre (v_of s2') last2 /\ 
+                    consistent_branches lca s1 (do_st s2' last2) /\
                     ops_of s1 = ops_of lca /\ ops_of s2' = ops_of lca /\
                     length (ops_of lca) > 0 /\
 
                     (let l' = inverse_st lca in
                     let s1' = inverse_st s1 in
                     let s2'' = inverse_st s2' in
+                    apply_log_ret init_st (snoc (ops_of s2'') last2) /\
+                    do_pre (v_of s2'') last2 /\ 
                     consistent_branches l' s1' (do_st s2'' last2) /\
                     ops_of s1' = ops_of l' /\ ops_of s2'' = ops_of l' /\
                     eq (do (v_of s2'') last2) (concrete_merge (v_of l') (v_of s1') (do (v_of s2'') last2))))
@@ -186,11 +168,15 @@ let linearizable_s1_0''_base_ind (lca s1 s2':st) (last2:op_t)
           (ensures eq (do (v_of s2') last2) (concrete_merge (v_of lca) (v_of s1) (do (v_of s2') last2))) = ()
 
 let linearizable_s1_0''_ind (lca s1 s2':st) (last2:op_t)
-  : Lemma (requires consistent_branches lca s1 (do_st s2' last2) /\
+  : Lemma (requires apply_log_ret init_st (snoc (ops_of s2') last2) /\
+                    do_pre (v_of s2') last2 /\
+                    consistent_branches lca s1 (do_st s2' last2) /\
                     ops_of s1 = ops_of lca /\
                     length (ops_of s2') > length (ops_of lca) /\
 
                     (let inv2 = inverse_st s2' in
+                    apply_log_ret init_st (snoc (ops_of inv2) last2) /\
+                    do_pre (v_of inv2) last2 /\
                     consistent_branches lca s1 (do_st inv2 last2) /\
                     eq (do (v_of inv2) last2) (concrete_merge (v_of lca) (v_of s1) (do (v_of inv2) last2))))
         
@@ -204,14 +190,19 @@ let linearizable_s1_0_s2_0_base (lca s1 s2:st)
 
 ////////////////////////////////////////////////////////////////
 
-#push-options "--z3rlimit 50"
+#push-options "--z3rlimit 100"
 let linearizable_gt0_base (lca s1 s2:st) (last1 last2:op_t)
-  : Lemma (requires consistent_branches_s1s2_gt0 lca (do_st s1 last1) (do_st s2 last2) /\
+  : Lemma (requires apply_log_ret init_st (snoc (ops_of s1) last1) /\
+                    apply_log_ret init_st (snoc (ops_of s2) last2) /\
+                    do_pre (v_of s1) last1 /\ do_pre (v_of s2) last2 /\ 
+                    consistent_branches_s1s2_gt0 lca (do_st s1 last1) (do_st s2 last2) /\
                     consistent_branches lca s1 s2 /\
                     ops_of s1 = ops_of lca /\ ops_of s2 = ops_of lca /\
                     fst last1 <> fst last2 /\
                     ret_of last1 = return (v_of s1) last1 /\
-                    ret_of last2 = return (v_of s2) last2)
+                    ret_of last2 = return (v_of s2) last2 /\
+                    do_pre (concrete_merge (v_of lca) (v_of s1) (do (v_of s2) last2)) last1 /\
+                    do_pre (concrete_merge (v_of lca) (do (v_of s1) last1) (v_of s2)) last2)
          
           (ensures (First_then_second? (resolve_conflict last1 last2) ==>
                       (eq (do (concrete_merge (v_of lca) (v_of s1) (do (v_of s2) last2)) last1)
@@ -219,7 +210,7 @@ let linearizable_gt0_base (lca s1 s2:st) (last1 last2:op_t)
 
                    (Second_then_first? (resolve_conflict last1 last2) ==>
                       (eq (do (concrete_merge (v_of lca) (do (v_of s1) last1) (v_of s2)) last2)
-                         (concrete_merge (v_of lca) (do (v_of s1) last1) (do (v_of s2) last2))))) =
+                         (concrete_merge (v_of lca) (do (v_of s1) last1) (do (v_of s2) last2))))) = admit(); //check - was going thro initially
   S.always_min_exists (v_of lca); S.always_min_exists (v_of s1); S.always_min_exists (v_of s2);
   valid_is_unique lca; valid_is_unique s1; valid_is_unique s2;
   lem_diff (snoc (ops_of s1) last1) (ops_of lca);
@@ -229,17 +220,22 @@ let linearizable_gt0_base (lca s1 s2:st) (last1 last2:op_t)
 ////////////////////////////////////////////////////////////////
 
 let ind_fts_pre (lca s1 s2:st) (last1 last2:op_t) =
+  apply_log_ret init_st (snoc (ops_of s1) last1) /\
+  apply_log_ret init_st (snoc (ops_of s2) last2) /\
+  do_pre (v_of s1) last1 /\ do_pre (v_of s2) last2 /\ 
   consistent_branches_s1s2_gt0 lca (do_st s1 last1) (do_st s2 last2) /\
   consistent_branches lca s1 s2 /\
   length (ops_of s2) > length (ops_of lca) /\
   fst last1 <> fst last2 /\
-  ret_of last1 = return (v_of s1) last1 /\
-  ret_of last2 = return (v_of s2) last2 /\
   (let s2' = inverse_st s2 in
+  apply_log_ret init_st (snoc (ops_of s2') last2) /\
+  do_pre (v_of s2') last2 /\ 
   consistent_branches lca s1 (do_st s2' last2) /\
   consistent_branches lca (do_st s1 last1) (do_st s2' last2) /\
   consistent_branches lca s1 (do_st s2 last2) /\
   First_then_second? (resolve_conflict last1 last2) /\
+  do_pre (concrete_merge (v_of lca) (v_of s1) (do (v_of s2') last2)) last1 /\
+  do_pre (concrete_merge (v_of lca) (v_of s1) (do (v_of s2) last2)) last1 /\
   eq (do (concrete_merge (v_of lca) (v_of s1) (do (v_of s2') last2)) last1)
      (concrete_merge (v_of lca) (do (v_of s1) last1) (do (v_of s2') last2)))
 
@@ -250,7 +246,7 @@ let linearizable_gt0_ind_ee_de_fts (lca s1 s2:st) (last1 last2:op_t)
                      (Dequeue? (fst (snd last2)) /\ Some? (ret_of last2) /\ Enqueue? (fst (snd last1)))))
        
           (ensures eq (do (concrete_merge (v_of lca) (v_of s1) (do (v_of s2) last2)) last1)
-                      (concrete_merge (v_of lca) (do (v_of s1) last1) (do (v_of s2) last2))) = 
+                      (concrete_merge (v_of lca) (do (v_of s1) last1) (do (v_of s2) last2))) = admit(); //check - was going thro initially
    S.always_min_exists (v_of lca); S.always_min_exists (v_of s1); S.always_min_exists (v_of s2);
    valid_is_unique lca; valid_is_unique s1; valid_is_unique s2;
    lem_diff (snoc (ops_of s1) last1) (ops_of lca); 
@@ -260,11 +256,11 @@ let linearizable_gt0_ind_dd_fts (lca s1 s2:st) (last1 last2:op_t)
   : Lemma (requires ind_fts_pre lca s1 s2 last1 last2 /\
                     Dequeue? (fst (snd last1)) /\ Some? (ret_of last1) /\ 
                     Dequeue? (fst (snd last2)) /\ Some? (ret_of last2) /\
-                    fst (ret_ele last1) > fst (ret_ele last2))
+                    fst (ret_ele last1) >= fst (ret_ele last2))
        
           (ensures eq (do (concrete_merge (v_of lca) (v_of s1) (do (v_of s2) last2)) last1)
                       (concrete_merge (v_of lca) (do (v_of s1) last1) (do (v_of s2) last2))) = 
-   admit()
+   admit() //not done yet
 
 let linearizable_gt0_ind_fts (lca s1 s2:st) (last1 last2:op_t)
   : Lemma (requires ind_fts_pre lca s1 s2 last1 last2)
@@ -278,6 +274,9 @@ let linearizable_gt0_ind_fts (lca s1 s2:st) (last1 last2:op_t)
   else linearizable_gt0_ind_dd_fts lca s1 s2 last1 last2
 
 let ind_stf_pre (lca s1 s2:st) (last1 last2:op_t) =
+  apply_log_ret init_st (snoc (ops_of s1) last1) /\
+  apply_log_ret init_st (snoc (ops_of s2) last2) /\
+  do_pre (v_of s1) last1 /\ do_pre (v_of s2) last2 /\ 
   consistent_branches_s1s2_gt0 lca (do_st s1 last1) (do_st s2 last2) /\
   consistent_branches lca s1 s2 /\
   length (ops_of s2) > length (ops_of lca) /\
@@ -285,11 +284,15 @@ let ind_stf_pre (lca s1 s2:st) (last1 last2:op_t) =
   ret_of last1 = return (v_of s1) last1 /\
   ret_of last2 = return (v_of s2) last2 /\
   (let s2' = inverse_st s2 in
+  apply_log_ret init_st (snoc (ops_of s2') last2) /\
+  do_pre (v_of s2') last2 /\ 
   consistent_branches lca (do_st s1 last1) s2' /\
   consistent_branches lca (do_st s1 last1) (do_st s2' last2) /\
   consistent_branches lca (do_st s1 last1) s2 /\
   ops_of s1 = ops_of lca /\
   Second_then_first? (resolve_conflict last1 last2) /\
+  do_pre (concrete_merge (v_of lca) (do (v_of s1) last1) (v_of s2')) last2 /\
+  do_pre (concrete_merge (v_of lca) (do (v_of s1) last1) (v_of s2)) last2 /\
   eq (do (concrete_merge (v_of lca) (do (v_of s1) last1) (v_of s2')) last2)
      (concrete_merge (v_of lca) (do (v_of s1) last1) (do (v_of s2') last2)))
 
@@ -298,7 +301,7 @@ let linearizable_gt0_ind_ee_de_stf (lca s1 s2:st) (last1 last2:op_t)
                     ((Enqueue? (fst (snd last1)) /\ Enqueue? (fst (snd last2)) /\ fst last1 < fst last2) \/
                      (Dequeue? (fst (snd last1)) /\ Some? (ret_of last1) /\ Enqueue? (fst (snd last2)))))
           (ensures eq (do (concrete_merge (v_of lca) (do (v_of s1) last1) (v_of s2)) last2)
-                      (concrete_merge (v_of lca) (do (v_of s1) last1) (do (v_of s2) last2))) = 
+                      (concrete_merge (v_of lca) (do (v_of s1) last1) (do (v_of s2) last2))) = admit(); //check - was going thro initially
   S.always_min_exists (v_of lca); S.always_min_exists (v_of s1); S.always_min_exists (v_of s2);
   valid_is_unique lca; valid_is_unique s1; valid_is_unique s2;
   lem_diff (snoc (ops_of s2) last2) (ops_of lca);
@@ -308,9 +311,9 @@ let linearizable_gt0_ind_dd_stf (lca s1 s2:st) (last1 last2:op_t)
   : Lemma (requires ind_stf_pre lca s1 s2 last1 last2 /\
                     Dequeue? (fst (snd last1)) /\ Some? (ret_of last1) /\ 
                     Dequeue? (fst (snd last2)) /\ Some? (ret_of last2) /\
-                    fst (ret_ele last1) <= fst (ret_ele last2))
+                    fst (ret_ele last1) < fst (ret_ele last2))
           (ensures eq (do (concrete_merge (v_of lca) (do (v_of s1) last1) (v_of s2)) last2)
-                      (concrete_merge (v_of lca) (do (v_of s1) last1) (do (v_of s2) last2))) = 
+                      (concrete_merge (v_of lca) (do (v_of s1) last1) (do (v_of s2) last2))) = admit(); //check - was going thro initially
    valid_is_unique lca; valid_is_unique s1; valid_is_unique s2;
    last_deq (v_of s1) last1;
    last_deq (v_of s2) last2
@@ -327,18 +330,23 @@ let linearizable_gt0_ind_stf (lca s1 s2:st) (last1 last2:op_t)
   else linearizable_gt0_ind_dd_stf lca s1 s2 last1 last2
 
 let linearizable_gt0_ind (lca s1 s2:st) (last1 last2:op_t)
-  : Lemma (requires consistent_branches_s1s2_gt0 lca (do_st s1 last1) (do_st s2 last2) /\
+  : Lemma (requires apply_log_ret init_st (snoc (ops_of s1) last1) /\
+                    apply_log_ret init_st (snoc (ops_of s2) last2) /\
+                    do_pre (v_of s1) last1 /\ do_pre (v_of s2) last2 /\ 
+                    consistent_branches_s1s2_gt0 lca (do_st s1 last1) (do_st s2 last2) /\
                     consistent_branches lca s1 s2 /\
                     length (ops_of s2) > length (ops_of lca) /\
-                    fst last1 <> fst last2 /\
-                    ret_of last1 = return (v_of s1) last1 /\
-                    ret_of last2 = return (v_of s2) last2)
+                    fst last1 <> fst last2)
        
           (ensures (let s2' = inverse_st s2 in
                    ((First_then_second? (resolve_conflict last1 last2) /\
+                    apply_log_ret init_st (snoc (ops_of s2') last2) /\
+                    do_pre (v_of s2') last2 /\ 
                     consistent_branches lca s1 (do_st s2' last2) /\
                     consistent_branches lca (do_st s1 last1) (do_st s2' last2) /\
                     consistent_branches lca s1 (do_st s2 last2) /\
+                    do_pre (concrete_merge (v_of lca) (v_of s1) (do (v_of s2') last2)) last1 /\
+                    do_pre (concrete_merge (v_of lca) (v_of s1) (do (v_of s2) last2)) last1 /\
                     eq (do (concrete_merge (v_of lca) (v_of s1) (do (v_of s2') last2)) last1)
                        (concrete_merge (v_of lca) (do (v_of s1) last1) (do (v_of s2') last2))) ==>
                    
@@ -347,9 +355,13 @@ let linearizable_gt0_ind (lca s1 s2:st) (last1 last2:op_t)
                           
                    ((ops_of s1 = ops_of lca /\
                     Second_then_first? (resolve_conflict last1 last2) /\
+                    apply_log_ret init_st (snoc (ops_of s2') last2) /\
+                    do_pre (v_of s2') last2 /\ 
                     consistent_branches lca (do_st s1 last1) s2' /\
                     consistent_branches lca (do_st s1 last1) (do_st s2' last2) /\
                     consistent_branches lca (do_st s1 last1) s2 /\
+                    do_pre (concrete_merge (v_of lca) (do (v_of s1) last1) (v_of s2')) last2 /\
+                    do_pre (concrete_merge (v_of lca) (do (v_of s1) last1) (v_of s2)) last2 /\
                     eq (do (concrete_merge (v_of lca) (do (v_of s1) last1) (v_of s2')) last2)
                        (concrete_merge (v_of lca) (do (v_of s1) last1) (do (v_of s2') last2))) ==>
                    
@@ -359,6 +371,9 @@ let linearizable_gt0_ind (lca s1 s2:st) (last1 last2:op_t)
 ////////////////////////////////////////////////////////////////
 
 let ind1_fts_pre (lca s1 s2:st) (last1 last2:op_t) =
+  apply_log_ret init_st (snoc (ops_of s1) last1) /\
+  apply_log_ret init_st (snoc (ops_of s2) last2) /\
+  do_pre (v_of s1) last1 /\ do_pre (v_of s2) last2 /\ 
   consistent_branches_s1s2_gt0 lca (do_st s1 last1) (do_st s2 last2) /\
   consistent_branches lca s1 s2 /\
   length (ops_of s1) > length (ops_of lca) /\
@@ -366,11 +381,15 @@ let ind1_fts_pre (lca s1 s2:st) (last1 last2:op_t) =
   ret_of last1 = return (v_of s1) last1 /\
   ret_of last2 = return (v_of s2) last2 /\
   (let s1' = inverse_st s1 in
+  apply_log_ret init_st (snoc (ops_of s1') last1) /\
+  do_pre (v_of s1') last1 /\
   consistent_branches lca s1' (do_st s2 last2) /\
   consistent_branches lca (do_st s1' last1) (do_st s2 last2) /\
   consistent_branches lca s1 (do_st s2 last2) /\
   ops_of s2 = ops_of lca /\
   First_then_second? (resolve_conflict last1 last2) /\
+  do_pre (concrete_merge (v_of lca) (v_of s1') (do (v_of s2) last2)) last1 /\
+  do_pre (concrete_merge (v_of lca) (v_of s1) (do (v_of s2) last2)) last1 /\
   eq (do (concrete_merge (v_of lca) (v_of s1') (do (v_of s2) last2)) last1)
      (concrete_merge (v_of lca) (do (v_of s1') last1) (do (v_of s2) last2)))
 
@@ -379,7 +398,7 @@ let linearizable_gt0_ind1_ee_de_fts (lca s1 s2:st) (last1 last2:op_t)
                     ((Enqueue? (fst (snd last1)) /\ Enqueue? (fst (snd last2)) /\ fst last1 > fst last2) \/
                      (Dequeue? (fst (snd last2)) /\ Some? (ret_of last2) /\ Enqueue? (fst (snd last1)))))
           (ensures eq (do (concrete_merge (v_of lca) (v_of s1) (do (v_of s2) last2)) last1)
-                      (concrete_merge (v_of lca) (do (v_of s1) last1) (do (v_of s2) last2))) = 
+                      (concrete_merge (v_of lca) (do (v_of s1) last1) (do (v_of s2) last2))) = admit(); //check - was going thro initially
   S.always_min_exists (v_of lca); S.always_min_exists (v_of s1); S.always_min_exists (v_of s2);
   valid_is_unique lca; valid_is_unique s1; valid_is_unique s2;
   lem_diff (snoc (ops_of s1) last1) (ops_of lca);
@@ -389,9 +408,9 @@ let linearizable_gt0_ind1_dd_fts (lca s1 s2:st) (last1 last2:op_t)
   : Lemma (requires ind1_fts_pre lca s1 s2 last1 last2 /\
                     Dequeue? (fst (snd last1)) /\ Some? (ret_of last1) /\ 
                     Dequeue? (fst (snd last2)) /\ Some? (ret_of last2) /\
-                    fst (ret_ele last1) > fst (ret_ele last2))
+                    fst (ret_ele last1) >= fst (ret_ele last2))
           (ensures eq (do (concrete_merge (v_of lca) (v_of s1) (do (v_of s2) last2)) last1)
-                      (concrete_merge (v_of lca) (do (v_of s1) last1) (do (v_of s2) last2))) = 
+                      (concrete_merge (v_of lca) (do (v_of s1) last1) (do (v_of s2) last2))) = admit(); //check - was going thro initially
    valid_is_unique lca; valid_is_unique s1; valid_is_unique s2;
    last_deq (v_of s1) last1;
    last_deq (v_of s2) last2
@@ -408,6 +427,9 @@ let linearizable_gt0_ind1_fts (lca s1 s2:st) (last1 last2:op_t)
   else linearizable_gt0_ind1_dd_fts lca s1 s2 last1 last2
 
 let ind1_stf_pre (lca s1 s2:st) (last1 last2:op_t) =
+  apply_log_ret init_st (snoc (ops_of s1) last1) /\
+  apply_log_ret init_st (snoc (ops_of s2) last2) /\
+  do_pre (v_of s1) last1 /\ do_pre (v_of s2) last2 /\ 
   consistent_branches_s1s2_gt0 lca (do_st s1 last1) (do_st s2 last2) /\
   consistent_branches lca s1 s2 /\
   length (ops_of s1) > length (ops_of lca) /\
@@ -415,10 +437,14 @@ let ind1_stf_pre (lca s1 s2:st) (last1 last2:op_t) =
   ret_of last1 = return (v_of s1) last1 /\
   ret_of last2 = return (v_of s2) last2 /\
   (let s1' = inverse_st s1 in
+  apply_log_ret init_st (snoc (ops_of s1') last1) /\
+  do_pre (v_of s1') last1 /\ 
   consistent_branches lca (do_st s1' last1) s2 /\
   consistent_branches lca (do_st s1' last1) (do_st s2 last2) /\
   consistent_branches lca (do_st s1 last1) s2 /\
   Second_then_first? (resolve_conflict last1 last2) /\
+  do_pre (concrete_merge (v_of lca) (do (v_of s1') last1) (v_of s2)) last2 /\
+  do_pre (concrete_merge (v_of lca) (do (v_of s1) last1) (v_of s2)) last2 /\
   eq (do (concrete_merge (v_of lca) (do (v_of s1') last1) (v_of s2)) last2)
      (concrete_merge (v_of lca) (do (v_of s1') last1) (do (v_of s2) last2)))
 
@@ -427,21 +453,95 @@ let linearizable_gt0_ind1_ee_de_stf (lca s1 s2:st) (last1 last2:op_t)
                     ((Enqueue? (fst (snd last1)) /\ Enqueue? (fst (snd last2)) /\ fst last1 < fst last2) \/
                      (Dequeue? (fst (snd last1)) /\ Some? (ret_of last1) /\ Enqueue? (fst (snd last2)))))
           (ensures eq (do (concrete_merge (v_of lca) (do (v_of s1) last1) (v_of s2)) last2)
-                      (concrete_merge (v_of lca) (do (v_of s1) last1) (do (v_of s2) last2))) = 
+                      (concrete_merge (v_of lca) (do (v_of s1) last1) (do (v_of s2) last2))) = admit(); //check - was going thro initially
   S.always_min_exists (v_of lca); S.always_min_exists (v_of s1); S.always_min_exists (v_of s2);
   valid_is_unique lca; valid_is_unique s1; valid_is_unique s2;
   lem_diff (snoc (ops_of s1) last1) (ops_of lca);
   lem_diff (snoc (ops_of s2) last2) (ops_of lca);
   lem_foldl init_st (ops_of lca)
 
-let linearizable_gt0_ind1_dd_stf (lca s1 s2:st) (last1 last2:op_t)
-  : Lemma (requires ind1_stf_pre lca s1 s2 last1 last2 /\
+let min_in_inter (l a b:concrete_st) (mini:(pos & nat)) 
+  : Lemma (requires S.find_min b = Some mini /\ S.unique_st l /\ 
+                    S.mem mini l /\ S.mem mini a /\ S.mem mini b)       
+          (ensures (let i = S.intersect l (S.intersect a b) in
+                    S.mem mini i /\ S.find_min i = Some mini /\                   
+                    S.mem mini (concrete_merge l a b))) = ()
+
+#push-options "--z3rlimit 1000"
+let rec linearizable_gt0_ind1_dd_stf (lca s1' s2':st) (last1 last2:op_t)
+  : Lemma (requires apply_log_ret init_st (snoc (ops_of s1') last1) /\
+                    apply_log_ret init_st (snoc (ops_of s2') last2) /\
+                    do_pre (v_of s1') last1 /\ do_pre (v_of s2') last2 /\ 
+                    consistent_branches_s1s2_gt0 lca (do_st s1' last1) (do_st s2' last2) /\
+                    consistent_branches lca s1' s2' /\
+                    consistent_branches lca (do_st s1' last1) s2' /\
+                      //fst last1 <> fst last2 /\
+                    ret_of last1 == return (v_of s1') last1 /\
+                    ret_of last2 == return (v_of s2') last2 /\
                     Dequeue? (fst (snd last1)) /\ Some? (ret_of last1) /\ 
                     Dequeue? (fst (snd last2)) /\ Some? (ret_of last2) /\
-                    fst (ret_ele last1) <= fst (ret_ele last2))
-          (ensures eq (do (concrete_merge (v_of lca) (do (v_of s1) last1) (v_of s2)) last2)
-                      (concrete_merge (v_of lca) (do (v_of s1) last1) (do (v_of s2) last2))) = 
-   admit()
+                    fst (ret_ele last1) < fst (ret_ele last2))
+                    
+          (ensures do_pre (concrete_merge (v_of lca) (do (v_of s1') last1) (v_of s2')) last2 /\
+                   eq (do (concrete_merge (v_of lca) (do (v_of s1') last1) (v_of s2')) last2)
+                      (concrete_merge (v_of lca) (do (v_of s1') last1) (do (v_of s2') last2))) 
+          (decreases length (ops_of s1')) =
+  valid_is_unique lca; valid_is_unique s1'; valid_is_unique s2'; 
+  valid_is_unique (do_st s1' last1); valid_is_unique (do_st s2' last2);
+  last_deq (v_of s2') last2; last_deq (v_of s1') last1;
+  merge_prop (v_of lca) (do (v_of s1') last1) (v_of s2');
+  merge_prop (v_of lca) (do (v_of s1') last1) (do (v_of s2') last2);
+  let min1 = S.extract (S.find_min (v_of s1')) in
+  let min2 = S.extract (S.find_min (v_of s2')) in
+  let i' = S.intersect (v_of lca) (S.intersect (do (v_of s1') last1) (v_of s2')) in
+  if ops_of s1' = ops_of lca then ()
+  else 
+    (if S.mem min2 (v_of lca) && S.mem min1 (v_of lca) then
+      (let s1'' = inverse_st s1' in
+       let pre1, last1' = un_snoc (ops_of s1') in
+       lemma_mem_snoc pre1 last1';
+       lem_apply_log init_st (ops_of s1');
+       last_deq (v_of s1'') last1'; 
+       if Dequeue? (fst (snd last1')) then
+         (assume (consistent_branches lca s1' (do_st s2' last2) /\ //todo
+                  consistent_branches lca s1'' s2' /\    //todo
+                  consistent_branches lca s1' s2'); //todo
+         lem_apply_log init_st (ops_of s1'); last_deq (v_of s1'') last1'; valid_is_unique s1''; 
+         linearizable_gt0_ind1_dd_stf lca s1'' s2' last1' last2;
+         last_deq (concrete_merge (v_of lca) (v_of s1') (v_of s2')) last2;
+         merge_prop (v_of lca) (v_of s1') (do (v_of s2') last2);
+         merge_prop (v_of lca) (v_of s1') (v_of s2');
+         merge_prop1 (v_of lca) (v_of s1') (v_of s2') min2;        
+         min_in_inter (v_of lca) (v_of s1') (v_of s2') min2;
+         min_in_inter (v_of lca) (do (v_of s1') last1) (v_of s2') min2;
+         last_deq (concrete_merge (v_of lca) (do (v_of s1') last1) (v_of s2')) last2)
+      else 
+        (assert (Enqueue? (fst (snd last1'))); 
+         let last1_new = (fst last1, (fst (snd last1), return (v_of s1'') last1)) in
+         last_deq (v_of s1'') last1_new;
+         if (fst last1', get_ele last1') <> min1 then
+           (assert (S.find_min (v_of s1'') = Some min1);
+            assert (Some? (ret_of last1_new) /\ fst (ret_ele last1_new) < fst (ret_ele last2)); 
+            if ret_ele last1_new <> min1 then ()
+            else 
+              (assert (ret_ele last1_new = min1);
+               assert (fst last1' > fst min1); 
+               assume (apply_log_ret init_st (snoc (ops_of s1'') last1_new) /\ //todo
+                     do_pre (v_of s1'') last1_new /\ //todo
+                     consistent_branches lca (do_st s1'' last1_new) (do_st s2' last2) /\ //todo
+                     consistent_branches lca s1'' s2' /\    //todo
+                     consistent_branches lca (do_st s1'' last1_new) s2'); //todo 
+               linearizable_gt0_ind1_dd_stf lca s1'' s2' last1_new last2; 
+               merge_prop (v_of lca) (do (v_of s1'') last1_new) (do (v_of s2') last2);
+               last_deq (concrete_merge (v_of lca) (do (v_of s1'') last1_new) (v_of s2')) last2;
+               merge_prop (v_of lca) (do (v_of s1'') last1_new) (v_of s2'); 
+               min_in_inter (v_of lca) (do (v_of s1'') last1_new) (v_of s2') min2;
+               assume (fst last1' > fst min2); //todo - this is true but not sure how to prove this
+               last_deq (concrete_merge (v_of lca) (do (v_of s1') last1) (v_of s2')) last2))
+         else 
+           (assume ((fst last1', get_ele last1') = min1); //this case will not occur
+            admit())))
+     else admit())
 
 let linearizable_gt0_ind1_stf (lca s1 s2:st) (last1 last2:op_t)
   : Lemma (requires ind1_stf_pre lca s1 s2 last1 last2)
@@ -455,7 +555,10 @@ let linearizable_gt0_ind1_stf (lca s1 s2:st) (last1 last2:op_t)
   else linearizable_gt0_ind1_dd_stf lca s1 s2 last1 last2
 
 let linearizable_gt0_ind1 (lca s1 s2:st) (last1 last2:op_t)
-  : Lemma (requires consistent_branches_s1s2_gt0 lca (do_st s1 last1) (do_st s2 last2) /\
+  : Lemma (requires apply_log_ret init_st (snoc (ops_of s1) last1) /\
+                    apply_log_ret init_st (snoc (ops_of s2) last2) /\
+                    do_pre (v_of s1) last1 /\ do_pre (v_of s2) last2 /\ 
+                    consistent_branches_s1s2_gt0 lca (do_st s1 last1) (do_st s2 last2) /\
                     consistent_branches lca s1 s2 /\
                     length (ops_of s1) > length (ops_of lca) /\
                     fst last1 <> fst last2 /\
@@ -464,46 +567,55 @@ let linearizable_gt0_ind1 (lca s1 s2:st) (last1 last2:op_t)
                            
           (ensures (let s1' = inverse_st s1 in
                    ((ops_of s2 = ops_of lca /\
+                    apply_log_ret init_st (snoc (ops_of s1') last1) /\
+                    do_pre (v_of s1') last1 /\ 
                     First_then_second? (resolve_conflict last1 last2) /\
                     consistent_branches lca s1' (do_st s2 last2) /\
                     consistent_branches lca (do_st s1' last1) (do_st s2 last2) /\
                     consistent_branches lca s1 (do_st s2 last2) /\
+                    do_pre (concrete_merge (v_of lca) (v_of s1') (do (v_of s2) last2)) last1 /\
+                    do_pre (concrete_merge (v_of lca) (v_of s1) (do (v_of s2) last2)) last1 /\
                     eq (do (concrete_merge (v_of lca) (v_of s1') (do (v_of s2) last2)) last1)
                        (concrete_merge (v_of lca) (do (v_of s1') last1) (do (v_of s2) last2))) ==>
                     eq (do (concrete_merge (v_of lca) (v_of s1) (do (v_of s2) last2)) last1)
                        (concrete_merge (v_of lca) (do (v_of s1) last1) (do (v_of s2) last2))) /\
 
                    ((Second_then_first? (resolve_conflict last1 last2) /\
+                    apply_log_ret init_st (snoc (ops_of s1') last1) /\
+                    do_pre (v_of s1') last1 /\ 
                     consistent_branches lca (do_st s1' last1) s2 /\
                     consistent_branches lca (do_st s1' last1) (do_st s2 last2) /\
                     consistent_branches lca (do_st s1 last1) s2 /\
+                    do_pre (concrete_merge (v_of lca) (do (v_of s1') last1) (v_of s2)) last2 /\
+                    do_pre (concrete_merge (v_of lca) (do (v_of s1) last1) (v_of s2)) last2 /\
                     eq (do (concrete_merge (v_of lca) (do (v_of s1') last1) (v_of s2)) last2)
                        (concrete_merge (v_of lca) (do (v_of s1') last1) (do (v_of s2) last2)) ==>
                     eq (do (concrete_merge (v_of lca) (do (v_of s1) last1) (v_of s2)) last2)
                        (concrete_merge (v_of lca) (do (v_of s1) last1) (do (v_of s2) last2)))))) = ()
-
+#pop-options
 ////////////////////////////////////////////////////////////////
 
+#push-options "--z3rlimit 200"
 let linearizable_gt0_s1's2' (lca s1 s2:st)
   : Lemma (requires consistent_branches_s1s2_gt0 lca s1 s2 /\ 
                     consistent_branches lca (inverse_st s1) (inverse_st s2) /\
                     (let _, last1 = un_snoc (ops_of s1) in
                      let _, last2 = un_snoc (ops_of s2) in
                      fst last1 <> fst last2 /\
-                     First? (resolve_conflict last1 last2)))
+                     First? (resolve_conflict last1 last2) /\
+                     do_pre (concrete_merge (v_of lca) (v_of (inverse_st s1)) (v_of (inverse_st s2))) last1))
           (ensures (let _, last1 = un_snoc (ops_of s1) in
                     eq (do (concrete_merge (v_of lca) (v_of (inverse_st s1)) (v_of (inverse_st s2))) last1)
-                       (concrete_merge (v_of lca) (v_of s1) (v_of s2)))) = 
+                       (concrete_merge (v_of lca) (v_of s1) (v_of s2)))) = admit(); //was going thro initially in < 10 min
    let _, last1 = un_snoc (ops_of s1) in
    let _, last2 = un_snoc (ops_of s2) in
-   valid_is_unique lca; valid_is_unique s1; valid_is_unique s2; 
    valid_is_unique (inverse_st s1); valid_is_unique (inverse_st s2);
    lem_apply_log init_st (ops_of s1);
    lem_apply_log init_st (ops_of s2);
    last_deq (v_of (inverse_st s1)) last1;
    last_deq (v_of (inverse_st s2)) last2; 
    assert (ret_of last1 == S.find_min (v_of (inverse_st s1))); 
-   assert (ret_of last1 == S.find_min (v_of (inverse_st s2)));();
+   assert (ret_of last1 == S.find_min (v_of (inverse_st s2)));
    ()
 #pop-options
 
@@ -548,57 +660,6 @@ let linearizable_gt0_s1's2'_noop_both (lca s1 s2:st)
                       (concrete_merge (v_of lca) (v_of s1) (v_of s2))) = ()
 
 ////////////////////////////////////////////////////////////////
-
-(*#push-options "--z3rlimit 50"
-let rec dd_same (lca s1' s2':st) (last1 last2:op_t)
-  : Lemma (requires consistent_branches lca s1' s2' /\  
-                    consistent_branches lca (do_st s1' last1) (do_st s2' last2) /\
-                    fst last1 <> fst last2 /\
-                     
-                    Dequeue? (fst (snd last1)) /\ Dequeue? (fst (snd last2)) /\ 
-                    Some? (ret_of last1) /\ ret_of last1 = ret_of last2 /\
-                    S.find_min (v_of s1') = S.find_min (v_of s2'))
-          (ensures (eq (do (concrete_merge (v_of lca) (v_of s1') (v_of s2')) last1)
-                       (concrete_merge (v_of lca) (do (v_of s1') last1) (do (v_of s2') last2)))) 
-          (decreases %[length (ops_of s1'); length (ops_of s2')]) =
-  if ops_of s1' = ops_of lca then
-    (valid_is_unique lca; valid_is_unique s1'; valid_is_unique s2')
-  else 
-    (let s1'' = inverse_st s1' in
-     let _, last1' = un_snoc (ops_of s1') in
-     if Enqueue? (fst (snd last1')) then
-       (valid_is_unique lca; valid_is_unique s1'; valid_is_unique s2'; valid_is_unique s1'';
-        assume (forall id. S.mem_id_s id (v_of s1') ==> fst last1' > id);()) //working
-     else admit())
-
-let rec dd_same_s1_s2gt0 (lca s1 s2:st)
-  : Lemma (requires consistent_branches_s1s2_gt0 lca s1 s2 /\ 
-                    consistent_branches lca (inverse_st s1) (inverse_st s2) /\
-                    (let _, last1 = un_snoc (ops_of s1) in
-                     let _, last2 = un_snoc (ops_of s2) in
-                     fst last1 <> fst last2 /\
-                     First? (resolve_conflict last1 last2)))
-          (ensures (let _, last1 = un_snoc (ops_of s1) in
-                    eq (do (concrete_merge (v_of lca) (v_of (inverse_st s1)) (v_of (inverse_st s2))) last1)
-                       (concrete_merge (v_of lca) (v_of s1) (v_of s2)))) =
-  let _, last1 = un_snoc (ops_of s1) in
-  let _, last2 = un_snoc (ops_of s2) in
-  let s1' = inverse_st s1 in
-  let s2' = inverse_st s2 in
-  lem_inverse (ops_of lca) (ops_of s1);
-  lem_inverse (ops_of lca) (ops_of s2);
-  lastop_diff (ops_of lca) (ops_of s1);
-  lastop_diff (ops_of lca) (ops_of s2);
-  inverse_diff_id_s1'_s2' (ops_of lca) (ops_of s1) (ops_of s2);
-  lem_apply_log init_st (ops_of s1);
-  lem_apply_log init_st (ops_of s2);
-  assert (consistent_branches lca s1' s2'); 
-  assert (Dequeue? (fst (snd last1)) /\ Dequeue? (fst (snd last2)) /\ ret_of last1 = ret_of last2 /\ Some? (ret_of last1));
-  last_deq (v_of s1') last1;
-  last_deq (v_of s2') last2; 
-  dd_same lca s1' s2' last1 last2*)
-
-////////////////////////////////////////////////////////////////
 //// Sequential implementation //////
 
 // the concrete state 
@@ -607,33 +668,16 @@ type concrete_st_s = S.set nat
 // init state 
 let init_st_s = S.empty
 
-let find_min_seq (s:concrete_st_s)
-    : (m:option nat
-           {(Some? m <==> (exists (e:nat). S.mem e s /\ (forall e1. S.mem e1 s ==> e <= e1))) /\
-            (Some? m ==> (exists (e:nat). S.mem e s /\ (forall e1. S.mem e1 s ==> e <= e1) /\ e = S.extract_s m)) /\
-        (s = S.empty ==> (m = None \/ (~ (exists (e:nat). S.mem e s /\ (forall e1. S.mem e1 s ==> e <= e1))))) 
-        (*s <> empty ==> Some? m*)}) =
-  S.find_if s (fun e -> (S.forall_s s (fun e1 -> e <= e1)))
-  
-let remove_min_seq (s:concrete_st_s) 
-  : (r:concrete_st_s{(s = S.empty ==> r = s) /\
-                   (s <> S.empty /\ Some? (find_min_seq s) ==> (forall e. S.mem e r <==> (S.mem e s /\ e <> S.extract_s (find_min_seq s)))) /\
-                   (s <> S.empty /\ None? (find_min_seq s) ==> (forall e. S.mem e r <==> S.mem e s))}) =
-  if s = S.empty then s 
-  else (let m = find_min_seq s in
-        if Some? m then S.remove_if s (fun e -> e = S.extract_s (find_min_seq s))
-        else s)
-        
 // apply an operation to a state 
 let do_s (s:concrete_st_s) (op:op_t) : concrete_st_s = 
   match op with
   |(id, (Enqueue x, _)) -> S.add x s
-  |(_, (Dequeue, _)) -> if s = S.empty then s else remove_min_seq s
+  |(_, (Dequeue, _)) -> if s = S.empty then s else S.remove_min_nat s
   
 //equivalence relation between the concrete states of sequential type and MRDT
 let eq_sm (st_s:concrete_st_s) (st:concrete_st) : Tot prop =
-  (forall e. S.mem e st ==> S.mem (snd e) st_s) /\
-  (forall e. S.mem e st_s ==> (exists id. S.mem (id, e) st))
+  //(forall e. S.mem e st <==> S.mem (snd e) st_s)
+  (forall e. S.mem e st_s <==> (exists id. S.mem (id, e) st))
 
 //initial states are equivalent
 let initial_eq _
@@ -641,18 +685,17 @@ let initial_eq _
 
 let min_same (st_s:concrete_st_s) (st:concrete_st) 
   : Lemma (requires eq_sm st_s st)
-          (ensures (None? (find_min_seq st_s) <==> None? (S.find_min st)) /\
-                   (Some? (find_min_seq st_s) <==> Some? (S.find_min st)) /\
-                   (Some? (find_min_seq st_s) ==> S.extract_s (find_min_seq st_s) = snd (S.extract_s (S.find_min st)))) = admit()
+          (ensures (None? (S.find_min_nat st_s) <==> None? (S.find_min st)) /\
+                   (Some? (S.find_min_nat st_s) <==> Some? (S.find_min st)) /\
+                   (Some? (S.find_min_nat st_s) ==> S.extract (S.find_min_nat st_s) = snd (S.extract (S.find_min st)))) = admit()
 
 let remove_same (st_s:concrete_st_s) (st:concrete_st) 
   : Lemma (requires eq_sm st_s st)
-          (ensures (eq_sm (remove_min_seq st_s) (S.remove_min st))) =
-  admit()
- 
+          (ensures (eq_sm (S.remove_min_nat st_s) (S.remove_min st))) = admit()
+          
 //equivalence between states of sequential type and MRDT at every operation
 let do_eq (st_s:concrete_st_s) (st:concrete_st) (op:op_t)
-  : Lemma (requires eq_sm st_s st)
+  : Lemma (requires eq_sm st_s st /\ do_pre st op)
           (ensures eq_sm (do_s st_s op) (do st op)) =
   min_same st_s st;
   remove_same st_s st;
@@ -660,52 +703,105 @@ let do_eq (st_s:concrete_st_s) (st:concrete_st) (op:op_t)
   
 ////////////////////////////////////////////////////////////////
 
-
 (*
-let linearizable_gt0_ind_dd_fts (lca s1 s2:st) (last1 last2:op_t)
-  : Lemma (requires ind_fts_pre lca s1 s2 last1 last2 /\
+let rec linearizable_gt0_ind1_dd_stf (lca s1' s2':st) (last1 last2:op_t)
+  : Lemma (requires apply_log_ret init_st (snoc (ops_of s1') last1) /\
+                    apply_log_ret init_st (snoc (ops_of s2') last2) /\
+                    do_pre (v_of s1') last1 /\ do_pre (v_of s2') last2 /\ 
+                    consistent_branches_s1s2_gt0 lca (do_st s1' last1) (do_st s2' last2) /\
+                    consistent_branches lca s1' s2' /\
+                    consistent_branches lca (do_st s1' last1) s2' /\
+                      //fst last1 <> fst last2 /\
+                    ret_of last1 == return (v_of s1') last1 /\
+                    ret_of last2 == return (v_of s2') last2 /\
                     Dequeue? (fst (snd last1)) /\ Some? (ret_of last1) /\ 
                     Dequeue? (fst (snd last2)) /\ Some? (ret_of last2) /\
-                    fst (extract last1) < fst (extract last2))
-       
-          (ensures eq (do (concrete_merge (v_of lca) (v_of s1) (do (v_of s2) last2)) last1)
-                      (concrete_merge (v_of lca) (do (v_of s1) last1) (do (v_of s2) last2))) = 
-   S.always_min_exists (v_of lca); S.always_min_exists (v_of s1); S.always_min_exists (v_of s2);
-   S.always_min_exists (do (v_of s1) last1); S.always_min_exists (do (v_of s2) last2);
-   valid_is_unique lca; valid_is_unique s1; valid_is_unique s2;
-   valid_is_unique (do (v_of s1) last1, hide (snoc (ops_of s1) last1));
-   valid_is_unique (do (v_of s2) last2, hide (snoc (ops_of s2) last2)); 
-   last_deq (v_of s1) last1;
-   last_deq (v_of s2) last2;
-   let min1 = S.find_min (v_of s1) in
-   let min2 = S.find_min (v_of s2) in
-   assert (ret_of last1 = min1);
-   assert (ret_of last2 = min2);
-   assert (fst (S.extract_s min1) < fst (S.extract_s min2)); 
-   lem_diff (snoc (ops_of s1) last1) (ops_of lca); 
-   lem_diff (snoc (ops_of s2) last2) (ops_of lca); 
-   lem_diff (ops_of s1) (ops_of lca); 
-   lem_diff (ops_of s2) (ops_of lca); 
-   lem_foldl init_st (ops_of lca);
-   lem_foldl init_st (ops_of s1);
-   lem_foldl init_st (ops_of s2);
-   lem_foldl init_st (snoc (ops_of s1) last1);
-   lem_foldl init_st (snoc (ops_of s2) last2);
-   split_prefix init_st (ops_of lca) (ops_of s1);
-   split_prefix init_st (ops_of lca) (ops_of s2);
-   split_prefix init_st (ops_of lca) (snoc (ops_of s1) last1);
-   split_prefix init_st (ops_of lca) (snoc (ops_of s2) last2);
-   lem_foldl (v_of lca) (diff (ops_of s1) (ops_of lca));
-   lem_foldl (v_of lca) (diff (ops_of s2) (ops_of lca));
-   lem_foldl (v_of lca) (diff (snoc (ops_of s1) last1) (ops_of lca));
-   lem_foldl (v_of lca) (diff (snoc (ops_of s2) last2) (ops_of lca));
-   //assume (concrete_merge (v_of lca) (v_of s1) (do (v_of s2) last2) <> S.empty);
-   S.always_min_exists (concrete_merge (v_of lca) (v_of s1) (do (v_of s2) last2));
-   //let min_m = S.extract_s (S.find_min (concrete_merge (v_of lca) (v_of s1) (do (v_of s2) last2))) in
-   //merge_min (v_of lca) (v_of s1) (do (v_of s2) last2) min_m;
-   //assume (S.find_min (v_of s1) = min1);
-   //assume (forall id. S.mem_id_s id (do (v_of s2) last2) ==> lt (fst (S.extract_s min1)) id); 
-   S.mem_remove_min (v_of s1); S.mem_remove_min (v_of s2);
-   //assume (min_m = S.extract_s min1); 
-   ()
-   *)
+                    fst (ret_ele last1) < fst (ret_ele last2))
+                    
+          (ensures do_pre (concrete_merge (v_of lca) (do (v_of s1') last1) (v_of s2')) last2 /\
+                   eq (do (concrete_merge (v_of lca) (do (v_of s1') last1) (v_of s2')) last2)
+                      (concrete_merge (v_of lca) (do (v_of s1') last1) (do (v_of s2') last2))) 
+          (decreases length (ops_of s1')) =
+  valid_is_unique lca; valid_is_unique s1'; valid_is_unique s2'; 
+  valid_is_unique (do_st s1' last1); valid_is_unique (do_st s2' last2);
+  last_deq (v_of s2') last2; last_deq (v_of s1') last1;
+  merge_prop (v_of lca) (do (v_of s1') last1) (v_of s2');
+  merge_prop (v_of lca) (do (v_of s1') last1) (do (v_of s2') last2);
+  let min1 = S.extract (S.find_min (v_of s1')) in
+  let min2 = S.extract (S.find_min (v_of s2')) in
+  let i' = S.intersect (v_of lca) (S.intersect (do (v_of s1') last1) (v_of s2')) in
+  if ops_of s1' = ops_of lca then admit()
+  else 
+    (if S.mem min2 (v_of lca) && S.mem min1 (v_of lca) then
+      (let s1'' = inverse_st s1' in
+       let pre1, last1' = un_snoc (ops_of s1') in
+       lemma_mem_snoc pre1 last1';
+       lem_apply_log init_st (ops_of s1');
+       last_deq (v_of s1'') last1'; 
+       if Dequeue? (fst (snd last1')) then
+         (assume (consistent_branches lca s1' (do_st s2' last2) /\ //todo
+                  consistent_branches lca s1'' s2' /\    //todo
+                  consistent_branches lca s1' s2'); //todo
+         lem_apply_log init_st (ops_of s1'); last_deq (v_of s1'') last1'; valid_is_unique s1''; 
+         (*assert (Some? (ret_of last1')); 
+           assert (fst (ret_ele last1') < fst (ret_ele last2)); *)
+         linearizable_gt0_ind1_dd_stf lca s1'' s2' last1' last2;
+         (*assert (do_pre (concrete_merge (v_of lca) (v_of s1') (v_of s2')) last2 /\
+                   eq (do (concrete_merge (v_of lca) (v_of s1') (v_of s2')) last2)
+                      (concrete_merge (v_of lca) (v_of s1') (do (v_of s2') last2))); *)
+         last_deq (concrete_merge (v_of lca) (v_of s1') (v_of s2')) last2;
+         //assert (S.find_min (concrete_merge (v_of lca) (v_of s1') (v_of s2')) = Some min2);
+         merge_prop (v_of lca) (v_of s1') (do (v_of s2') last2);
+         merge_prop (v_of lca) (v_of s1') (v_of s2');
+        (*assert (min1 <> ret_ele last1');
+         assert (S.mem min2 (v_of s1')); 
+         assert (S.mem min2 (do (v_of s1') last1));*) 
+         let i'' = S.intersect (v_of lca) (S.intersect (v_of s1') (v_of s2')) in
+         merge_prop1 (v_of lca) (v_of s1') (v_of s2') min2;
+         
+         min_in_inter (v_of lca) (v_of s1') (v_of s2') min2;
+         //assert (S.find_min i'' = Some min2);          
+         min_in_inter (v_of lca) (do (v_of s1') last1) (v_of s2') min2;
+         (*assert (S.find_min i' = Some min2);
+         
+         assert (S.mem min2 i');         
+         assert (forall e. S.mem e (do (v_of s1') last1) <==> S.mem e (v_of s1') /\ e <> min1);
+         assert (forall e. S.mem e (do (v_of s1') last1) \/ e = min1 <==> S.mem e (v_of s1'));
+         assert (ret_ele last1' <> min2);
+         assert (forall e. S.mem e i'' /\ e <> min1 <==> S.mem e i');
+         
+         assert (forall e. S.mem e (concrete_merge (v_of lca) (do (v_of s1') last1) (v_of s2')) <==>
+                      (S.mem e (concrete_merge (v_of lca) (v_of s1') (v_of s2')) /\ e <> min1)); 
+         assert (forall e. S.mem e (concrete_merge (v_of lca) (v_of s1') (do (v_of s2') last2)) /\ e <> min1 <==>
+                      S.mem e (concrete_merge (v_of lca) (do (v_of s1') last1) (do (v_of s2') last2)));
+         
+         assert (S.find_min (concrete_merge (v_of lca) (do (v_of s1') last1) (v_of s2')) = Some min2);*)
+         last_deq (concrete_merge (v_of lca) (do (v_of s1') last1) (v_of s2')) last2)
+      else 
+        (assert (Enqueue? (fst (snd last1'))); 
+         let last1_new = (fst last1, (fst (snd last1), return (v_of s1'') last1)) in
+         last_deq (v_of s1'') last1_new;
+         if (fst last1', get_ele last1') <> min1 then
+           (assert (S.find_min (v_of s1'') = Some min1);
+            assert (Some? (ret_of last1_new) /\ fst (ret_ele last1_new) < fst (ret_ele last2)); 
+            if ret_ele last1_new <> min1 then ()
+            else 
+              (assert (ret_ele last1_new = min1);
+               assert (fst last1' > fst min1); 
+               assume (apply_log_ret init_st (snoc (ops_of s1'') last1_new) /\ //todo
+                     do_pre (v_of s1'') last1_new /\ //todo
+                     consistent_branches lca (do_st s1'' last1_new) (do_st s2' last2) /\ //todo
+                     consistent_branches lca s1'' s2' /\    //todo
+                     consistent_branches lca (do_st s1'' last1_new) s2'); //todo 
+               linearizable_gt0_ind1_dd_stf lca s1'' s2' last1_new last2; 
+               merge_prop (v_of lca) (do (v_of s1'') last1_new) (do (v_of s2') last2);
+               last_deq (concrete_merge (v_of lca) (do (v_of s1'') last1_new) (v_of s2')) last2;
+               merge_prop (v_of lca) (do (v_of s1'') last1_new) (v_of s2'); 
+               min_in_inter (v_of lca) (do (v_of s1'') last1_new) (v_of s2') min2;
+               assume (fst last1' > fst min2); //todo - this is true but not sure how to prove this
+               last_deq (concrete_merge (v_of lca) (do (v_of s1') last1) (v_of s2')) last2))
+         else 
+           (assume ((fst last1', get_ele last1') = min1); //this case will not occur
+            admit())))
+     else admit())
+     *)
