inductive_proof/Queue_set/Set_extended.fst
@@ -17,14 +17,12 @@ let equal (#a:eqtype) (s1:set a) (s2:set a) =
 let equal_mem (#a:eqtype) (s1:set a) (s2:set a)
   : Lemma (ensures (equal s1 s2 <==> (forall e. mem e s1 <==> mem e s2))) = ()
 
-let singleton (#a:eqtype) (x:a) = [x]
+let add (#a:eqtype) (ele:a) (s:set a) = 
+  if mem ele s then s else ele::s
 
-let singleton_mem (#a:eqtype) (x:a) (y:a) 
-  : Lemma (ensures (mem y (singleton x) = (x=y))) = ()
-
-let add (#a:eqtype) (ele:a) (s:set a) = ele::s
-
-let add_mem (#a:eqtype) (ele:a) (s:set a) (x:a) = ()
+let add_mem (#a:eqtype) (ele:a) (s:set a) (x:a)
+  : Lemma (ensures (mem ele s ==> (add ele s == s)) /\
+                   (not (mem ele s) ==> (mem x (add ele s) <==> (mem x s \/ x == ele)))) = ()
 
 let union (#a:eqtype) (s1:set a) (s2:set a) =
   List.Tot.Base.append s1 s2
@@ -44,7 +42,7 @@ let rec intersect (#a:eqtype) (s1:set a) (s2:set a) =
   |x::xs -> if mem x s2 then x::intersect xs (remove x s2) else intersect xs s2
   
 let rec intersect_mem (#a:eqtype) (s1:set a) (s2:set a) (x:a)
-  : Lemma (ensures mem x (intersect s1 s2) <==> (mem x s1 /\ mem x s2)) 
+  : Lemma (ensures mem x (intersect s1 s2) <==> (mem x s1 /\ mem x s2))
     (decreases s1) =
   match s1 with
   |[] -> ()
@@ -56,7 +54,7 @@ let rec remove_if (#a:eqtype) (s:set a) (f:a -> bool) =
   |x::xs -> if f x then remove_if xs f else x::remove_if xs f
 
 let rec remove_if_mem (#a:eqtype) (s:set a) (f:a -> bool) (x:a)
-  : Lemma (ensures mem x (remove_if s f) <==> (mem x s /\ ~ (f x))) = 
+  : Lemma (ensures mem x (remove_if s f) <==> (mem x s /\ ~ (f x))) =
   match s with
   |[] -> ()
   |x1::xs -> remove_if_mem xs f x
@@ -94,7 +92,7 @@ let rec forall_mem (#a:eqtype) (s:set a) (f:a -> bool)
   |[] -> ()
   |x::xs -> forall_mem xs f
 
-let extr (#a:eqtype) (x:option a{Some? x}) : (r:a{x = Some r}) =
+let extract (#a:Type0) (x:option a{Some? x}) : (r:a{x == Some r}) =
   let (Some a) = x in a
 
 let rec find_if (#a:eqtype) (s:set a) (f:a -> bool) : option a =
@@ -105,7 +103,7 @@ let rec find_if (#a:eqtype) (s:set a) (f:a -> bool) : option a =
 let rec mem_find_if (#a:eqtype) (s:set a) (f:a -> bool)
   : Lemma (ensures (None? (find_if s f) <==> ((forall e. mem e s ==> ~ (f e)) \/ s = empty)) /\
                    (Some? (find_if s f) <==> (exists e. mem e s /\ f e)) /\
-                   (Some? (find_if s f) ==> (exists e. mem e s /\ f e /\ e = extr (find_if s f)) /\ (f (extr (find_if s f))))) = 
+                   (Some? (find_if s f) ==> (exists e. mem e s /\ f e /\ e = extract (find_if s f)) /\ (f (extract (find_if s f))))) = 
   match s with
   |[] -> ()
   |x::xs -> if f x then () else mem_find_if xs f
@@ -114,7 +112,7 @@ let rec mem_find_if_exists (#a:eqtype) (s:set a) (f:a -> bool)
   : Lemma (requires (exists e. mem e s /\ f e))
           (ensures (None? (find_if s f) <==> ((forall e. mem e s ==> ~ (f e)) \/ s = empty)) /\
                    (Some? (find_if s f) <==> (exists e. mem e s /\ f e)) /\
-                   (Some? (find_if s f) ==> (exists e. mem e s /\ f e /\ e = extr (find_if s f)) /\ (f (extr (find_if s f)))) /\
+                   (Some? (find_if s f) ==> (exists e. mem e s /\ f e /\ e = extract (find_if s f)) /\ (f (extract (find_if s f)))) /\
                    (s <> empty ==> Some? (find_if s f))) = 
   match s with
   |[] -> ()
@@ -126,30 +124,81 @@ let rec always_min_exists (#a:eqtype) (s:set (pos * a))
   |[] -> ()
   |x::xs -> always_min_exists xs
 
-let extract_s (#a:Type0) (m:option a{Some? m}) =
-  let (Some x) = m in x
-
 let find_min (#a:eqtype) (s:set (pos * a))
   : (m:option (pos * a)
            {(Some? m <==> (exists (e:(pos * a)). mem e s /\ (forall e1. mem e1 s ==> fst e <= fst e1))) /\
-            (Some? m ==> (exists (e:(pos * a)). mem e s /\ (forall e1. mem e1 s ==> fst e <= fst e1) /\ e = extract_s m)) /\
-        (s = empty ==> (m = None \/ (~ (exists (e:(pos * a)). mem e s /\ (forall e1. mem e1 s ==> fst e <= fst e1)))))}) =
+            (Some? m <==> (exists (e:(pos * a)). mem e s /\ (forall e1. mem e1 s ==> fst e <= fst e1) /\ e = extract m)) /\
+            (s = empty <==> m = None) /\
+            (Some? m ==> mem (extract m) s)}) =
+  always_min_exists s;
   find_if s (fun e -> (forall_s s (fun e1 -> fst e <= fst e1)))
 
 let mem_find_min (#a:eqtype) (s:set (pos * a))
   : Lemma (ensures (Some? (find_min s) <==> (exists (e:(pos * a)). mem e s /\ (forall e1. mem e1 s ==> fst e <= fst e1))) /\
-            (Some? (find_min s) ==> (exists (e:(pos * a)). mem e s /\ (forall e1. mem e1 s ==> fst e <= fst e1) /\ e = extract_s (find_min s))) /\
-        (s = empty ==> (find_min s = None \/ (~ (exists (e:(pos * a)). mem e s /\ (forall e1. mem e1 s ==> fst e <= fst e1)))))) = ()
+            (Some? (find_min s) <==> (exists (e:(pos * a)). mem e s /\ (forall e1. mem e1 s ==> fst e <= fst e1) /\ e = extract (find_min s))) /\
+            (s = empty <==> find_min s = None) /\
+            (Some? (find_min s) ==> mem (extract (find_min s)) s)) = 
+  always_min_exists s
 
 let remove_min (#a:eqtype) (s:set (pos * a)) 
-  : (r:set (pos * a){(s = empty ==> r = s) /\
-                   (s <> empty /\ Some? (find_min s) ==> (forall e. mem e r <==> (mem e s /\ e <> extract_s (find_min s)))) (*/\
+  : (r:set (pos * a){(s = empty <==> r = s) /\
+                   (s <> empty /\ Some? (find_min s) ==> (forall e. mem e r <==> (mem e s /\ e <> extract (find_min s)))) (*/\
                    (s <> empty /\ None? (find_min s) ==> (forall e. mem e r <==> mem e s)*)}) =
   always_min_exists s;
   if s = empty then s 
   else (let m = find_min s in
-        remove_if s (fun e -> e = extract_s (find_min s)))
+        remove_if s (fun e -> e = extract (find_min s)))
+
+let mem_remove_min (#a:eqtype) (s:set (pos * a)) 
+  : Lemma (ensures (let r = remove_min s in
+                   (s = empty <==> r = s) /\
+                   (s <> empty /\ Some? (find_min s) ==> (forall e. mem e r <==> (mem e s /\ e <> extract (find_min s)))) /\
+                   (s <> empty /\ None? (find_min s) ==> (forall e. mem e r <==> mem e s)))) = 
+  always_min_exists s
 
 let mem_id_s (#a:eqtype) (id:pos) (s:set (pos * a)) 
   : (b:bool{b = true <==> (exists e. mem e s /\ fst e = id)}) =
   exists_s s (fun e -> fst e = id)
+
+let same_uni (#a:eqtype) (s1 s2:set (pos & a)) (min1:(pos & a))
+  : Lemma (requires unique_st s1 /\ (forall e. mem e s2 <==> mem e s1 /\ e <> min1))
+          (ensures unique_st s2) = ()
+  
+let rec always_min_exists_nat (s:set nat) 
+  : Lemma (ensures (s <> empty ==> (exists (e:nat). mem e s /\ (forall (e1:nat). mem e1 s ==> e <= e1)))) =
+  match s with
+  |[] -> ()
+  |x::xs -> always_min_exists_nat xs
+  
+let find_min_nat (s:set nat)
+  : (m:option nat
+           {(Some? m <==> (exists (e:nat). mem e s /\ (forall e1. mem e1 s ==> e <= e1))) /\
+            (Some? m <==> (exists (e:nat). mem e s /\ (forall e1. mem e1 s ==> e <= e1) /\ e = extract m)) /\
+            (s = empty <==> m = None) /\
+            (Some? m ==> mem (extract m) s)}) =
+  always_min_exists_nat s;
+  find_if s (fun e -> (forall_s s (fun e1 -> e <= e1)))
+  
+let mem_find_min_nat (s:set nat)
+  : Lemma (ensures (Some? (find_min_nat s) <==> (exists (e:nat). mem e s /\ (forall e1. mem e1 s ==> e <= e1))) /\
+            (Some? (find_min_nat s) <==> (exists (e:nat). mem e s /\ (forall e1. mem e1 s ==> e <= e1) /\ e = extract (find_min_nat s))) /\
+            (s = empty <==> find_min_nat s = None) /\
+            (Some? (find_min_nat s) ==> mem (extract (find_min_nat s)) s)) = 
+  always_min_exists_nat s
+        
+let remove_min_nat (s:set nat)
+  : (r:set nat{(s = empty <==> r = s) /\
+                   (s <> empty /\ Some? (find_min_nat s) ==> (forall e. mem e r <==> (mem e s /\ e <> extract (find_min_nat s)))) (*/\
+                   (s <> empty /\ None? (find_min s) ==> (forall e. mem e r <==> mem e s)*)}) =
+  always_min_exists_nat s;
+  if s = empty then s 
+  else (let m = find_min_nat s in
+        remove_if s (fun e -> e = extract (find_min_nat s)))
+
+let mem_remove_min_nat (s:set nat)
+  : Lemma (ensures (let r = remove_min_nat s in
+                   (s = empty <==> r = s) /\
+                   (s <> empty /\ Some? (find_min_nat s) ==> (forall e. mem e r <==> (mem e s /\ e <> extract (find_min_nat s)))) /\
+                   (s <> empty /\ None? (find_min_nat s) ==> (forall e. mem e r <==> mem e s)))) = 
+  always_min_exists_nat s
+  
