inductive_proof/Queue_set/Set_extended.fsti
@@ -14,16 +14,12 @@ val equal_mem (#a:eqtype) (s1:set a) (s2:set a)
   : Lemma (ensures (equal s1 s2 <==> (forall e. mem e s1 <==> mem e s2)))
     [SMTPat (equal s1 s2)]
 
-val singleton (#a:eqtype) (x:a) : set a
-val singleton_mem (#a:eqtype) (x:a) (y:a) 
-  : Lemma (ensures (mem y (singleton x) = (x=y)))
-    [SMTPat (mem y (singleton x))]
-
 val add (#a:eqtype) (ele:a) (s:set a) : set a
 val add_mem (#a:eqtype) (ele:a) (s:set a) (x:a)
-  : Lemma (ensures mem x (add ele s) <==> (mem x s \/ x == ele))
+  : Lemma (ensures (mem ele s ==> (add ele s == s)) /\
+                   (not (mem ele s) ==> (mem x (add ele s) <==> (mem x s \/ x == ele))))
     [SMTPat (mem x (add ele s))]
-
+    
 val union (#a:eqtype) (s1:set a) (s2:set a) : set a
 val union_mem (#a:eqtype) (s1:set a) (s2:set a) (x:a)
   : Lemma (ensures mem x (union s1 s2) <==> (mem x s1 \/ mem x s2))
@@ -54,47 +50,99 @@ val forall_mem (#a:eqtype) (s:set a) (f:a -> bool)
   : Lemma (ensures ((forall_s s f = true) <==> (forall x. mem x s ==> f x)))
     [SMTPat (forall_s s f)]
 
-val extr (#a:eqtype) (x:option a{Some? x}) : (r:a{x = Some r})
+val extract (#a:Type0) (x:option a{Some? x}) : (r:a{x == Some r})
 
 val find_if (#a:eqtype) (s:set a) (f:a -> bool) : option a
 val mem_find_if (#a:eqtype) (s:set a) (f:a -> bool)
   : Lemma (ensures (None? (find_if s f) <==> ((forall e. mem e s ==> ~ (f e)) \/ s = empty)) /\
                    (Some? (find_if s f) <==> (exists e. mem e s /\ f e)) /\
-                   (Some? (find_if s f) ==> (exists e. mem e s /\ f e /\ e = extr (find_if s f)) /\ (f (extr (find_if s f)))))
+                   (Some? (find_if s f) ==> (exists e. mem e s /\ f e /\ e = extract (find_if s f)) /\ (f (extract (find_if s f)))))
     [SMTPat (find_if s f)]
 
 val mem_find_if_exists (#a:eqtype) (s:set a) (f:a -> bool)
   : Lemma (requires (exists e. mem e s /\ f e))
           (ensures (None? (find_if s f) <==> ((forall e. mem e s ==> ~ (f e)) \/ s = empty)) /\
                    (Some? (find_if s f) <==> (exists e. mem e s /\ f e)) /\
-                   (Some? (find_if s f) ==> (exists e. mem e s /\ f e /\ e = extr (find_if s f)) /\ (f (extr (find_if s f)))) /\
+                   (Some? (find_if s f) ==> (exists e. mem e s /\ f e /\ e = extract (find_if s f)) /\ (f (extract (find_if s f)))) /\
                    (s <> empty ==> Some? (find_if s f)))
           [SMTPat (find_if s f)]
 
 val always_min_exists (#a:eqtype) (s:set (pos * a)) 
   : Lemma (ensures (s <> empty ==> (exists (e:(pos * a)). mem e s /\ (forall (e1:(pos * a)). mem e1 s ==> fst e <= fst e1))))
 
-val extract_s (#a:Type0) (m:option a{Some? m}) : (e:a{m == Some e})
 
-val find_min (#a:eqtype) (s:set (pos * a)) 
+(*val find_min (#a:eqtype) (s:set (pos * a)) 
   : (m:option (pos * a)
      {(Some? m <==> (exists (e:(pos * a)). mem e s /\ (forall e1. mem e1 s ==> fst e <= fst e1))) /\
-            (Some? m ==> (exists (e:(pos * a)). mem e s /\ (forall e1. mem e1 s ==> fst e <= fst e1) /\ e = extract_s m)) /\
-        (s = empty ==> (m = None \/ (~ (exists (e:(pos * a)). mem e s /\ (forall e1. mem e1 s ==> fst e <= fst e1))))) })
+            (Some? m <==> (exists (e:(pos * a)). mem e s /\ (forall e1. mem e1 s ==> fst e <= fst e1) /\ e = extract_s m)) /\
+            (s = empty <==> m = None) /\
+            (Some? m ==> mem (extract_s m) s)})
 
 val mem_find_min (#a:eqtype) (s:set (pos * a))
   : Lemma (ensures (Some? (find_min s) <==> (exists (e:(pos * a)). mem e s /\ (forall e1. mem e1 s ==> fst e <= fst e1))) /\
-            (Some? (find_min s) ==> (exists (e:(pos * a)). mem e s /\ (forall e1. mem e1 s ==> fst e <= fst e1) /\ e = extract_s (find_min s))) /\
-        (s = empty ==> (find_min s = None \/ (~ (exists (e:(pos * a)). mem e s /\ (forall e1. mem e1 s ==> fst e <= fst e1)))))) 
-        [SMTPat (find_min s)]
+            (Some? (find_min s) <==> (exists (e:(pos * a)). mem e s /\ (forall e1. mem e1 s ==> fst e <= fst e1) /\ e = extract_s (find_min s))) /\
+            (s = empty <==> find_min s = None) /\
+            (Some? (find_min s) ==> mem (extract_s (find_min s)) s)) 
+        [SMTPat (find_min s)]*)
+
+val find_min (#a:eqtype) (s:set (pos * a)) 
+  : (m:option (pos * a){(Some? m <==> (exists (e:(pos * a)). mem e s /\ (forall e1. mem e1 s ==> fst e <= fst e1))) /\
+         (Some? m <==> (exists (e:(pos * a)). (mem e s /\ (forall e1. (mem e1 s /\ fst e <> fst e1) ==> fst e < fst e1) /\ e = extract m))) /\
+                        (s = empty <==> m = None) /\
+                        (Some? m ==> mem (extract m) s)})
+
+val mem_find_min (#a:eqtype) (s:set (pos * a))
+  : Lemma (ensures (Some? (find_min s) <==> (exists (e:(pos * a)). mem e s /\ (forall e1. mem e1 s ==> fst e <= fst e1))) /\
+     (Some? (find_min s) <==> (exists (e:(pos * a)). (mem e s /\ (forall e1. (mem e1 s /\ fst e <> fst e1) ==> fst e < fst e1) /\
+                            e = extract (find_min s)))) /\
+            (s = empty <==> find_min s = None) /\
+            (Some? (find_min s) ==> mem (extract (find_min s)) s))
 
 let unique_st (#a:eqtype) (s:set (pos * a)) =
   forall_s s (fun e -> not (exists_s s (fun e1 -> snd e <> snd e1 && fst e = fst e1)))
 
 val remove_min (#a:eqtype) (s:set (pos * a)) 
-  : (r:set (pos * a){(s = empty ==> r = s) /\
-                   (s <> empty /\ Some? (find_min s) ==> (forall e. mem e r <==> (mem e s /\ e <> extract_s (find_min s)))) /\
+  : (r:set (pos * a){(s = empty <==> r = s) /\
+                   (s <> empty /\ Some? (find_min s) ==> (forall e. mem e r <==> (mem e s /\ e <> extract (find_min s)))) /\
                    (s <> empty /\ None? (find_min s) ==> (forall e. mem e r <==> mem e s))})
+
+val mem_remove_min (#a:eqtype) (s:set (pos * a)) 
+  : Lemma (ensures (let r = remove_min s in
+                   (s = empty <==> r = s) /\
+                   (s <> empty /\ Some? (find_min s) ==> (forall e. mem e r <==> (mem e s /\ e <> extract (find_min s)))) /\
+                   (s <> empty /\ None? (find_min s) ==> (forall e. mem e r <==> mem e s))))
+    [SMTPat (remove_min s)]
 
 val mem_id_s (#a:eqtype) (id:pos) (s:set (pos * a)) 
   : (b:bool{b = true <==> (exists e. mem e s /\ fst e = id)})
+
+val same_uni (#a:eqtype) (s1 s2:set (pos & a)) (min1:(pos & a))
+  : Lemma (requires unique_st s1 /\ (forall e. mem e s2 <==> mem e s1 /\ e <> min1))
+          (ensures unique_st s2)
+
+val always_min_exists_nat (s:set nat) 
+  : Lemma (ensures (s <> empty ==> (exists (e:nat). mem e s /\ (forall (e1:nat). mem e1 s ==> e <= e1))))
+  
+val find_min_nat (s:set nat) : (m:option nat
+           {(Some? m <==> (exists (e:nat). mem e s /\ (forall e1. mem e1 s ==> e <= e1))) /\
+            (Some? m <==> (exists (e:nat). mem e s /\ (forall e1. mem e1 s ==> e <= e1) /\ e = extract m)) /\
+            (s = empty <==> m = None) /\
+            (Some? m ==> mem (extract m) s)})
+  
+val mem_find_min_nat (s:set nat)
+  : Lemma (ensures (Some? (find_min_nat s) <==> (exists (e:nat). mem e s /\ (forall e1. mem e1 s ==> e <= e1))) /\
+            (Some? (find_min_nat s) <==> (exists (e:nat). mem e s /\ (forall e1. mem e1 s ==> e <= e1) /\ e = extract (find_min_nat s))) /\
+            (s = empty <==> find_min_nat s = None) /\
+            (Some? (find_min_nat s) ==> mem (extract (find_min_nat s)) s))
+        
+val remove_min_nat (s:set nat)
+  : (r:set nat{(s = empty <==> r = s) /\
+                   (s <> empty /\ Some? (find_min_nat s) ==> (forall e. mem e r <==> (mem e s /\ e <> extract (find_min_nat s)))) (*/\
+                   (s <> empty /\ None? (find_min s) ==> (forall e. mem e r <==> mem e s)*)})
+
+val mem_remove_min_nat (s:set nat)
+  : Lemma (ensures (let r = remove_min_nat s in
+                   (s = empty <==> r = s) /\
+                   (s <> empty /\ Some? (find_min_nat s) ==> (forall e. mem e r <==> (mem e s /\ e <> extract (find_min_nat s)))) /\
+                   (s <> empty /\ None? (find_min_nat s) ==> (forall e. mem e r <==> mem e s))))
+                   
